specs/ecdsap256/Spec.P256.fst
@@ -6,9 +6,6 @@ open Lib.ByteSequence
 open Lib.IntTypes
 open Lib.Sequence
 
-open Spec.P256.Definitions
-open Spec.P256.Lemmas
-
 open FStar.Math.Lemmas
 open FStar.Math.Lib
 
@@ -16,7 +13,74 @@ open FStar.Math.Lib
 
 (* https://eprint.iacr.org/2013/816.pdf *)
 
-let prime = prime256
+
+let prime256: (a: pos {a > 3 && a < pow2 256}) =
+  assert_norm (pow2 256 - pow2 224 + pow2 192 + pow2 96 -1 > 3);
+  assert_norm (pow2 256 - pow2 224 + pow2 192 + pow2 96 -1 < pow2 256);
+  pow2 256 - pow2 224 + pow2 192 + pow2 96 -1
+
+
+let point_nat = tuple3 nat nat nat
+
+let point_nat_prime = (p: point_nat {let (a, b, c) = p in a < prime256 /\ b < prime256 /\ c < prime256})
+
+type elem (n:pos) = x:nat{x < n}
+
+let fmul (#n:pos) (x:elem n) (y:elem n) : elem n = (x * y) % n
+
+noextract
+val pow: a:nat -> b:nat -> nat
+
+let rec pow a b =
+  if b = 0 then 1
+  else a * (pow a (b - 1))
+
+
+#push-options "--fuel 1"
+
+noextract
+val pow_plus: a: nat -> b: nat -> c: nat -> 
+  Lemma (ensures (pow a b * pow a c = pow a (b + c))) 
+  (decreases b)
+
+let rec pow_plus a b c = 
+  match b with 
+  | 0 -> assert_norm (pow a 0 = 1)
+  | _ -> pow_plus a (b - 1) c
+
+#pop-options
+
+val exp: #n: pos -> a: elem n -> b: pos -> Tot (elem n) (decreases b)
+
+let rec exp #n a b =
+  if b = 1 then a
+  else
+    if b % 2 = 0 then exp (fmul a a) (b / 2)
+    else fmul a (exp (fmul a a) (b / 2))
+
+
+noextract
+let modp_inv_prime (prime: pos {prime > 3}) (x: elem prime) : Tot (elem prime) =
+  (exp #prime x (prime - 2)) % prime
+
+noextract
+let modp_inv2_prime (x: int) (p: nat {p > 3}) : Tot (elem p) = modp_inv_prime p (x % p)
+
+noextract
+let modp_inv2 (x: nat) : Tot (elem prime256) =
+  assert_norm(prime256 > 3);
+  modp_inv2_prime x prime256
+
+noextract
+let modp_inv2_pow (x: nat) : Tot (elem prime256) =
+   pow x (prime256 - 2) % prime256
+
+
+noextract
+let min_one_prime (prime: pos {prime > 3}) (x: int) : Tot (elem prime) =
+  let p = x % prime in 
+  exp #prime p (prime - 1)
+  
 
 let aCoordinateP256 = -3 
 let bCoordinateP256 : (a: nat {a < prime256}) =
@@ -38,10 +102,11 @@ let _point_double (p:point_nat_prime) : point_nat_prime =
   let gamma = y * y in 
   let beta = x * gamma in 
   let alpha = 3 * (x - delta) * (x + delta) in 
-  let x3 = (alpha * alpha - 8 * beta) % prime in 
-  let y3 = (alpha *  (4 * beta - x3) - 8 * gamma * gamma) % prime in 
-  let z3 = ((y + z) * (y + z) - delta - gamma) % prime in 
+  let x3 = (alpha * alpha - 8 * beta) % prime256 in 
+  let y3 = (alpha *  (4 * beta - x3) - 8 * gamma * gamma) % prime256 in 
+  let z3 = ((y + z) * (y + z) - delta - gamma) % prime256 in 
   (x3, y3, z3)
+
 
 noextract
 let _point_add (p:point_nat_prime) (q:point_nat_prime) : point_nat_prime =
@@ -96,22 +161,6 @@ let _norm (p:point_nat_prime) : point_nat_prime =
 let scalar = lbytes 32
 
 
-val lemma_scalar_ith: sc:lbytes 32 -> k:nat{k < 32} -> Lemma
-  (v sc.[k] == nat_from_intseq_le sc / pow2 (8 * k) % pow2 8)
-
-let lemma_scalar_ith sc k =
-  index_nat_to_intseq_le #U8 #SEC 32 (nat_from_intseq_le sc) k;
-  nat_from_intseq_le_inj sc (nat_to_intseq_le 32 (nat_from_intseq_le sc))
-
-
-val lemma_euclidian_for_ithbit: k: nat -> i: nat
-  -> Lemma (k / (pow2 (8 * (i / 8)) * pow2 (i % 8)) == k / pow2 i)
-
-let lemma_euclidian_for_ithbit k i =
-  lemma_div_def i 8;
-  pow2_plus (8 * (i / 8)) (i % 8)
-
-
 let ith_bit (k:lbytes 32) (i:nat{i < 256}) : uint64 =
   let q = 31 - i / 8 in let r = size (i % 8) in
   to_u64 ((index k q >>. r) &. u8 1)
@@ -148,11 +197,13 @@ let _ml_step k i (p, q) =
 
 val montgomery_ladder_spec: k:scalar -> tuple2 point_nat_prime point_nat_prime
   -> tuple2 point_nat_prime point_nat_prime
+
 let montgomery_ladder_spec k pq =
   Lib.LoopCombinators.repeati 256 (_ml_step k) pq
 
 
 val scalar_multiplication: scalar -> point_nat_prime -> point_nat_prime
+
 let scalar_multiplication k p =
   let pai = (0, 0, 0) in
   let q, f = montgomery_ladder_spec k (pai, p) in
@@ -160,6 +211,7 @@ let scalar_multiplication k p =
 
 
 val secret_to_public: scalar -> point_nat_prime
+
 let secret_to_public k =
   let pai = (0, 0, 0) in
   let q, f = montgomery_ladder_spec k (pai, basePoint) in
@@ -167,80 +219,13 @@ let secret_to_public k =
 
 
 val isPointOnCurve: point_nat_prime -> bool
+
 let isPointOnCurve p =
   let (x, y, z) = p in
-  (y * y) % prime =
-  (x * x * x + aCoordinateP256 * x + bCoordinateP256) % prime
-
-
-let point_prime_to_coordinates (p:point_seq) =
-  felem_seq_as_nat (Lib.Sequence.sub p 0 4),
-  felem_seq_as_nat (Lib.Sequence.sub p 4 4),
-  felem_seq_as_nat (Lib.Sequence.sub p 8 4)
+  (y * y) % prime256 =
+  (x * x * x + aCoordinateP256 * x + bCoordinateP256) % prime256
 
 
 val toJacobianCoordinates: tuple2 nat nat -> tuple3 nat nat nat
+
 let toJacobianCoordinates (r0, r1) = (r0, r1, 1)
-
-
-#push-options "--ifuel 1"
-
-val nat_from_intlist_le: #t:inttype{unsigned t} -> #l:secrecy_level -> list (uint_t t l) -> nat
-
-let rec nat_from_intlist_le #t #l = function
-  | [] -> 0
-  | hd :: tl -> v hd + pow2 (bits t) * nat_from_intlist_le tl
-
-val nat_from_intlist_be: #t:inttype{unsigned t} -> #l:secrecy_level -> list (uint_t t l) -> nat
-
-let rec nat_from_intlist_be #t #l = function
-  | [] -> 0
-  | hd :: tl -> pow2 (FStar.List.Tot.Base.length tl * bits t) * v hd + nat_from_intlist_be tl
-
-#pop-options
-
-#push-options "--fuel 1"
-
-val index_seq_of_list_cons: #a:Type -> x:a -> l:list a -> i:nat{i < List.Tot.length l} -> Lemma
-  (Seq.index (Seq.seq_of_list (x::l)) (i+1) == Seq.index (Seq.seq_of_list l) i)
-
-let index_seq_of_list_cons #a x l i =
-  assert (Seq.index (Seq.seq_of_list (x::l)) (i+1) == List.Tot.index (x::l) (i+1))
-
-val nat_from_intlist_seq_le: #t:inttype{unsigned t} -> #l:secrecy_level
-  -> len:size_nat -> b:list (uint_t t l){List.Tot.length b = len}
-  -> Lemma (nat_from_intlist_le b == nat_from_intseq_le (of_list b))
-
-let rec nat_from_intlist_seq_le #t #l len b =
-  match b with
-  | [] -> ()
-  | hd :: tl ->
-    begin
-    let s = of_list b in
-    Classical.forall_intro (index_seq_of_list_cons hd tl);
-    assert (equal (of_list tl) (slice s 1 len));
-    assert (index s 0 == List.Tot.index b 0);
-    nat_from_intseq_le_lemma0 (slice s 0 1);
-    nat_from_intseq_le_slice_lemma s 1;
-    nat_from_intlist_seq_le (len - 1) tl
-    end
-
-val nat_from_intlist_seq_be: #t: inttype {unsigned t} -> #l: secrecy_level
-  -> len: size_nat -> b: list (uint_t t l) {FStar.List.Tot.Base.length b = len}
-  -> Lemma (nat_from_intlist_be b == nat_from_intseq_be (of_list b))
-
-let rec nat_from_intlist_seq_be #t #l len b =
-  match b with
-  | [] -> ()
-  | hd :: tl ->
-    begin
-      let s = of_list b in
-      Classical.forall_intro (index_seq_of_list_cons hd tl);
-      assert (equal (of_list tl) (slice s 1 len));
-      assert (index s 0 == List.Tot.index b 0);
-      nat_from_intlist_seq_be (len - 1) tl;
-      nat_from_intseq_be_lemma0 (slice s 0 1);
-      nat_from_intseq_be_slice_lemma s 1
-      end
-
-#pop-options
